update lpzk proof

proof/src/zero-knowledge/definitions/sigma-protocol/ASigmaProtocol.ec
@@ -29,63 +29,35 @@ theory SigmaProtocol.
   type verifier_state_t.
 
   type commit_t.
-  type commit_op_t = prover_rand_t -> prover_input_t -> prover_state_t * commit_t.
-  op commit : commit_op_t.
+  op commit : prover_rand_t -> prover_input_t -> prover_state_t * commit_t.
   op valid_commit : commit_t -> bool.
 
   type challenge_t.
-  type challenge_op_t = verifier_rand_t -> verifier_input_t -> commit_t -> verifier_state_t * challenge_t.
-  op challenge : challenge_op_t.
+  op challenge : verifier_rand_t -> verifier_input_t -> commit_t -> verifier_state_t * challenge_t.
   op valid_challenge : challenge_t -> bool.
 
   type response_t.
-  type response_op_t = prover_state_t -> challenge_t -> prover_output_t * response_t.
-  op response : response_op_t.
+  op response : prover_state_t -> challenge_t -> prover_output_t * response_t.
   op valid_response : response_t -> bool.
 
-  type decide_op_t = verifier_state_t -> response_t -> verifier_output_t.
-  op decide : decide_op_t.
+  op decide : verifier_state_t -> response_t -> verifier_output_t.
 
-  type sigma_protocol_t = commit_op_t * challenge_op_t * response_op_t * decide_op_t.
   (** 3-message zk protocol *)
 
   type trace_t = commit_t * challenge_t * response_t.
 
-  op protocol (r : rand_t) (x : input_t) : (trace_t * output_t) option =
+  op protocol (r : rand_t) (x : input_t) : trace_t * output_t =
     let (rp, rv) = r in
     let (xp, xv) = x in
     let (stp, c) = commit rp xp in
-    if (valid_commit c) then
-      let (stv, ch) = challenge rv xv c in
-      if (valid_challenge ch) then
-        let (y1, resp) = response stp ch in
-        if (valid_response resp) then
-          let y2 = decide stv resp in
-          Some ((c, ch, resp), (y1, y2))
-        else None
-      else None
-    else None.
-
-  op run_protocol (r : rand_t) (x : input_t) (prot : sigma_protocol_t) : (trace_t * output_t) option =
-    let (rp, rv) = r in
-    let (xp, xv) = x in
-    let (commit, challenge, response, decide) = prot in
-    let (stp, c) = commit rp xp in
-    if (valid_commit c) then
-      let (stv, ch) = challenge rv xv c in
-      if (valid_challenge ch) then
-        let (y1, resp) = response stp ch in
-        if (valid_response resp) then
-          let y2 = decide stv resp in
-          Some ((c, ch, resp), (y1, y2))
-        else None
-      else None
-    else None.
+    let (stv, ch) = challenge rv xv c in
+    let (y1, resp) = response stp ch in
+    let y2 = decide stv resp in
+    ((c, ch, resp), (y1, y2)).
 
   axiom correct (r : rand_t) (x : input_t) :
     valid_rands r x =>
     valid_inputs x =>
-    protocol r x <> None =>
-    snd (oget (protocol r x)) = ((), relation (fst (fst x)) (snd x)).    
+    snd (protocol r x) = ((), relation (fst (fst x)) (snd x)).    
 
 end SigmaProtocol.
