proof/src/zero-knowledge/definitions/sigma-protocol/Completeness.ec
@@ -13,17 +13,13 @@ theory Completeness.
   module Completeness(R : Rand_t) = {
     proc main(w : witness_t, x : statement_t) : bool = {
       var r_p, r_v;
-      var tr, y, b, otry;
+      var tr, y, b;
 
       (r_p, r_v) <@ R.gen();
 
       if (valid_inputs ((w,x),x) /\ valid_rands (r_p, r_v) ((w,x),x)) {
-        otry <- protocol (r_p, r_v) ((w,x), x);
-        if (otry <> None) {
-          (tr,y) <- oget otry;
-          b <- (snd y);
-        }
-        else { b <- true; }
+        (tr,y) <- protocol (r_p, r_v) ((w,x), x);
+        b <- (snd y);
       }
       else { b <- true; (*{0,1};*) }
 
